add more sanity check

Examples/MerkleTree/SanityChecks.lean
@@ -4,10 +4,21 @@ import DY.Meta
 import DY.Meta.Utils
 public import Examples.MerkleTree.Specification
 public import Examples.MerkleTree.Proof
+import all Examples.MerkleTree.Proof
 public import Examples.MerkleTree.Instance
 public meta import Examples.MerkleTree.Instance
 
 namespace DY.Example.MerkleTree
+
+-- TODO: move, but where?
+theorem liftM_parse_preserves_reachability
+  {a: Type} [Comparse.ParseableSerializeable a]
+  (config: ReachabilityConfig)
+  (buf: Bytes)
+  : (liftM (Comparse.parse buf): Traceful a).PreservesReachability config (fun _ => True) (fun res _ => Comparse.FormatRel buf res)
+:= by
+  simp only [Traceful.PreservesReachability, Traceful.PreservesReachabilityFrom, liftM, monadLift, MonadLift.monadLift, Traceful.run_mk]
+  grind
 
 public
 def honestAttacker: Traceful Unit := do
@@ -114,5 +125,157 @@ info: 'DY.Example.MerkleTree.honestAttacker_properties' depends on axioms: [prop
 -/
 #guard_msgs in
 #print axioms honestAttacker_properties
+
+public
+def compromiseSigKeyAttacker: Traceful Unit := do
+  let (_, pkHandle, skHandle) ← LongTermKeys.generateKeyPair "MerkleTree PKI" "Bob" -- 4
+
+  let compromiseHandle ← LongTermKeys.compromisePrivateKey "MerkleTree PKI" skHandle -- 2
+  let globalStSigkeyBytes ← Network.receiveMessage compromiseHandle
+  let globalStSigkey: PersistentLocalState.LocalState (LongTermKeys.SecretKeyState "SignedDH PKI") ← Comparse.parse globalStSigkeyBytes
+  let sigKey := globalStSigkey.state.sk
+
+
+  let msg0 := (Literal.literalToBytes "foo 0".toByteArray)
+  let msg1 := (Literal.literalToBytes "bar 1".toByteArray)
+  let msg2 := (Literal.literalToBytes "baz 2".toByteArray)
+  let msg3 := (Literal.literalToBytes "qux 3".toByteArray)
+  let msg4 := (Literal.literalToBytes "quux 4".toByteArray)
+  let elements := [msg0, msg1, msg2, msg3, msg4, msg4]
+
+  let rootHash := merkleTreeHash (.bytes) elements
+  let tbs: SignedRootHashTBS := { rootHash, length := elements.length }
+  let tbsBytes: Bytes := Comparse.serialize tbs
+  let sigNonce := Literal.literalToBytes "00000000000000000000000000000000".toByteArray
+  let sig := Signature.sign sigKey sigNonce tbsBytes
+
+  let msgSig: SignedRootHash := { tbs, sig }
+  let msgSigHandle ← Network.sendMessage (Comparse.serialize msgSig)
+
+  let msgIncl: ElementAndInclusionProof := {
+    element := elements[4]
+    i := 4
+    inclusionProof := mkInclusionProof (.bytes) elements 4 (by grind)
+  }
+  let msgInclHandle ← Network.sendMessage (Comparse.serialize msgIncl)
+
+  Client.checkInclusion "Bob" msgSigHandle msgInclHandle pkHandle -- 1
+  return ()
+
+#guard (compromiseSigKeyAttacker.run Trace.nil).fst = some ()
+
+theorem compromiseSigKeyAttacker_PreservesReachability
+  : compromiseSigKeyAttacker.PreservesReachability reachability (fun _ => True) (fun _ _ => True)
+:= by
+  unfold Traceful.PreservesReachability
+  intro tr h_tr h_pre
+  dsimp only [compromiseSigKeyAttacker]
+
+  apply Traceful.PreservesReachabilityFrom_bind
+  · apply Traceful.PreservesReachability_base (LongTermKeys.generateKeyPair.reachability "MerkleTree PKI")
+  · assumption
+  · simp [LongTermKeys.generateKeyPair.reachability]
+  intro ⟨ _, pkHandle, skHandle ⟩ tr h_post h_tr h_le
+
+  apply Traceful.PreservesReachabilityFrom_bind
+  · apply Traceful.PreservesReachability_base (LongTermKeys.compromisePrivateKey.reachability "MerkleTree PKI")
+  · assumption
+  · simp [LongTermKeys.compromisePrivateKey.reachability]
+  intro compromiseHandle tr h_post h_tr h_le
+
+  apply Traceful.PreservesReachabilityFrom_bind
+  · apply Network.receiveMessage.preservesReachability
+  · assumption
+  · grind
+  intro globalStSigkeyBytes tr h_post h_tr h_le
+
+  apply Traceful.PreservesReachabilityFrom_bind
+  · apply liftM_parse_preserves_reachability
+  · assumption
+  · grind
+  intro globalStSigkey tr h_post h_tr h_le
+
+  apply Traceful.PreservesReachabilityFrom_bind
+  · apply Traceful.PreservesReachability_base (Network.reachability)
+  · assumption
+  · simp only [Comparse.AttackerKnows_serialize, SignedRootHash.IsWellFormed_eq]
+    apply And.intro
+    · simp only [SignedRootHashTBS.IsWellFormed_eq]
+      apply pred_merkleTreeHash _ _ (Bytes.AttackerKnows · tr)
+      · intro b h_b
+        apply Hash.attacker_knows_hash
+        grind
+      simp [Literal.attacker_knows_literalToBytes]
+    apply Signature.attacker_knows_sign
+    · grind
+    · apply Literal.attacker_knows_literalToBytes
+    · simp only [Comparse.AttackerKnows_serialize, SignedRootHashTBS.IsWellFormed_eq]
+      apply pred_merkleTreeHash _ _ (Bytes.AttackerKnows · tr)
+      · intro b h_b
+        apply Hash.attacker_knows_hash
+        grind
+      simp [Literal.attacker_knows_literalToBytes]
+  intro msgSigHandle tr h_post h_tr h_le
+
+  apply Traceful.PreservesReachabilityFrom_bind
+  · apply Traceful.PreservesReachability_base (Network.reachability)
+  · assumption
+  · simp only [Comparse.AttackerKnows_serialize, ElementAndInclusionProof.IsWellFormed_eq]
+    apply And.intro
+    · simp [Literal.attacker_knows_literalToBytes]
+    apply pred_mkInclusionProof _ _ _ _ (Bytes.AttackerKnows · tr)
+    · intro b h_b
+      apply Hash.attacker_knows_hash
+      grind
+    simp [Literal.attacker_knows_literalToBytes]
+  intro msgInclHandle tr h_post h_tr h_le
+
+  dsimp
+  apply Traceful.PreservesReachabilityFrom_bind
+  · apply Traceful.PreservesReachability_base (Client.checkInclusion.reachability) _ ("Bob", msgSigHandle, msgInclHandle, pkHandle)
+  · assumption
+  · simp [Client.checkInclusion.reachability]
+  intro _ tr h_post h_tr h_le
+
+  apply Traceful.PreservesReachabilityFrom_pure
+  · assumption
+  grind
+
+theorem rewrite_forall_nat_into_forall_fin {P: Nat → Prop} (n: Nat) (h: ∀ i, n ≤ i → P i): (∀ i: Nat, P i) = (∀ i: Fin n, P i.val) := by
+  simp only [eq_iff_iff]
+  constructor
+  · grind
+  · intro h i
+    by_cases n ≤ i
+    · grind
+    · exact h ⟨ i, by grind ⟩
+
+public
+theorem compromiseSigKeyAttacker_properties:
+  let tr := (compromiseSigKeyAttacker.run (Trace.nil)).snd.val
+  tr.Reachable reachability ∧
+  ∃ t1 element,
+    tr.EventLoggedAt (TheEvent.ClientAccept "Bob" element) t1 ∧
+    (∀ t2, ¬ (tr.EventLoggedAt (TheEvent.ServerAuthenticated "Bob" element) t2))
+:= by
+  intro tr
+  refine ⟨ ?_, ?_ ⟩
+  · apply Traceful.PreservesReachability_to_Reachable compromiseSigKeyAttacker_PreservesReachability
+    grind
+  conv in (∀ t': Nat, _) =>
+    rewrite [rewrite_forall_nat_into_forall_fin tr.length (by sorry)] -- sorry filled in ACME PR
+  simp only [DY.Trace.EventLoggedAt_eq_getEventAt]
+  refine ⟨ 8, (Literal.literalToBytes "quux 4".toByteArray), ?_ ⟩
+  native_decide
+
+/--
+info: 'DY.Example.MerkleTree.compromiseSigKeyAttacker_properties' depends on axioms: [propext,
+ sorryAx,
+ Classical.choice,
+ Quot.sound,
+ compromiseSigKeyAttacker_properties._native.native_decide.ax_1_2]
+-/
+#guard_msgs in
+#print axioms compromiseSigKeyAttacker_properties
 
 end DY.Example.MerkleTree
